unfair medium can now be modeled using overlap

abp/generated/abp/MediumStates.thy
@@ -3,7 +3,7 @@
  * This file was generated from Medium.maa and will be overridden when changed. To change
  * permanently, consider changing the model itself.
  *
- * Generated on Oct 16, 2018 10:17:27 PM by isartransformer 3.1.0
+ * Generated on Oct 16, 2018 10:34:43 PM by isartransformer 3.1.0
  *)
 theory MediumStates
   imports MediumDatatype
@@ -15,15 +15,11 @@ begin
 datatype MediumSubstate = Single
 
 (* And these have also the variables *)
-datatype MediumState = MediumState MediumSubstate (* coin = *) "int"
+datatype MediumState = MediumState MediumSubstate 
 
 (* Function to get the substate *)
 fun getMediumSubState :: "MediumState \<Rightarrow> MediumSubstate" where
-    "getMediumSubState (MediumState s _) = s"
-
-(* Functions to get the variables *)
-fun getCoin :: "MediumState \<Rightarrow> int" where
-"getCoin (MediumState _ var_coin) = var_coin"
+    "getMediumSubState (MediumState s ) = s"
 
 
 end
